Got subst of TPOSR and Right refl yay

proof/TPOSR/CtxCoercion.v
@@ -9,7 +9,6 @@ Require Import Lambda.TPOSR.Env.
 Require Import Lambda.TPOSR.TypesNoDerivs.
 Require Import Lambda.TPOSR.Thinning.
 Require Import Lambda.TPOSR.LeftReflexivity.
-Require Import Lambda.TPOSR.Substitution.
 
 Set Implicit Arguments.
 
@@ -19,7 +18,7 @@ Implicit Types A B M N T t u v : lterm.
 Implicit Types e f g : lenv.
 
 Inductive coerce_in_env : lenv -> lenv -> Prop :=
-  | coerce_env_hd : forall e t u s, e |-- t >-> u : s -> e |-- u -> u : Srt_l s ->
+  | coerce_env_hd : forall e t u s, e |-- t >-> u : s -> e |-- t -> t : s -> e |-- u -> u : Srt_l s ->
 	coerce_in_env (t :: e) (u :: e)
   | coerce_env_tl :
       forall e f t, coerce_in_env e f -> 
@@ -58,9 +57,9 @@ exists s ; auto with coc core.
 change (Srt_l s) with (llift 1 (Srt_l s)).
 split.
 apply thinning_n_coerce with l ; auto with coc core ;
-apply wf_cons with u s ; auto.
+apply wf_cons with s ; eauto with coc.
 apply thinning_n with l ; auto with coc core ;
-apply wf_cons with u s ; auto.
+apply wf_cons with s ; auto.
 
 left.
 exists x; auto with coc core arith datatypes.
@@ -111,9 +110,9 @@ change (Srt_l x2) with (llift 1 (Srt_l x2)).
 destruct H7.
 split.
 eapply thinning_n_coerce ; auto with coc core ;
-apply wf_cons with y s ; auto.
+apply wf_cons with s ; auto.
 eapply thinning_n ; auto with coc core ;
-apply wf_cons with y s ; auto.
+apply wf_cons with s ; auto.
 
 exists x; auto with coc core arith datatypes.
 Qed.
@@ -176,8 +175,8 @@ apply tposr_pi2_red with A' s1 B' s2 s3 u' ; eauto with coc.
 inversion H.
 inversion H0.
 subst.
-apply wf_cons with u s0 ; auto.
-apply wf_cons with A s0 ; auto.
+apply wf_cons with s0 ; auto.
+apply wf_cons with s0 ; auto.
 
 apply tposr_eq_trans with X ; auto with coc.
 
@@ -205,3 +204,116 @@ Lemma coerce_coerce_env : forall e T U s, e |-- T >-> U : s ->
 Proof (proj2 (proj2 (proj2 ind_coerce_env))).
 
 Hint Resolve tposr_coerce_env eq_coerce_env coerce_coerce_env : ecoc.
+
+Inductive coerce_in_env_full : lenv -> lenv -> Prop :=
+  | coerce_env_trans : forall e f g, coerce_in_env_full e f -> coerce_in_env_full f g -> coerce_in_env_full e g
+  | coerce_env_in_env : forall e f, coerce_in_env e f -> coerce_in_env_full e f
+  | coerce_env_nil : coerce_in_env_full nil nil.
+
+Hint Resolve coerce_env_in_env coerce_env_nil : coc.
+
+Lemma coerce_env_sym : forall e f, coerce_in_env e f -> coerce_in_env f e.
+Proof.
+  induction 1 ; simpl ; intros ; auto with coc.
+  apply coerce_env_hd with s ; eauto with coc.
+  apply coerce_env_tl with s ; eauto with coc.
+  apply tposr_coerce_env with f ; auto.
+Qed.  
+
+Lemma coerce_env_full_sym : forall e f, coerce_in_env_full e f -> coerce_in_env_full f e.
+Proof.
+  induction 1 ; simpl ; intros ; eauto with coc.
+  apply coerce_env_trans with f ; auto.
+  apply coerce_env_in_env ; auto.
+  apply coerce_env_sym ; auto.
+Qed.
+
+Hint Resolve coerce_env_sym coerce_env_full_sym : coc.
+
+Lemma coerce_env_full :
+  (forall e t u T, e |-- t -> u : T -> 
+  forall f, coerce_in_env_full e f -> f |-- t -> u : T).
+Proof.
+  intros.
+  induction H0 ; auto.
+
+  apply tposr_coerce_env with e ; auto with coc.
+Qed.
+
+Lemma coerce_env_full_cons : forall G D, coerce_in_env_full G D -> forall T, tposr_wf (T :: G) ->
+  coerce_in_env_full (T :: G) (T :: D).
+Proof.
+  induction 1 ; simpl ; intros.
+  apply coerce_env_trans with (T :: f) ; eauto with coc.
+  apply IHcoerce_in_env_full2.
+  inversion H1.
+  apply wf_cons with  s.
+  apply coerce_env_full with e ; auto with coc.
+
+  inversion H0.
+  subst.
+  apply coerce_env_in_env ; eauto with coc.
+
+  apply coerce_env_in_env ; auto with coc.
+  inversion H.
+  assert(nil |-- T -> T : s).
+  eauto with coc.
+  apply coerce_env_hd with s ; auto with coc.
+Qed.
+
+Corollary tposrp_coerce_env_full : 
+  (forall e t u T, e |-- t -+> u : T -> 
+  forall f, coerce_in_env_full e f -> f |-- t -+> u : T).
+Proof.
+  induction 1 ; simpl ; intros ; auto with coc.
+  apply tposrp_tposr ; eapply coerce_env_full ; eauto with coc.
+  apply tposrp_trans with X ; auto with coc.
+Qed.
+
+Corollary eq_coerce_env_full : 
+  (forall e t u s, e |-- t ~= u : s -> 
+  forall f, coerce_in_env_full e f -> f |-- t ~= u : s).
+Proof.
+  induction 1 ; simpl ; intros ; auto with coc.
+  apply tposr_eq_tposr ; eapply coerce_env_full ; eauto with coc.
+  apply tposr_eq_trans with X ; auto with coc.
+Qed.
+
+Hint Resolve coerce_env_full eq_coerce_env_full : ecoc.
+
+Corollary coerce_coerce_env_full : 
+  (forall e t u s, e |-- t >-> u : s -> 
+  forall f, coerce_in_env_full e f -> f |-- t >-> u : s).
+Proof.
+  induction 1 ; simpl ; intros ; auto with coc.
+
+  apply tposr_coerce_conv ; eapply eq_coerce_env_full ; eauto with coc.
+
+  assert(coerce_in_env_full (A' :: e) (A' :: f)) by
+  (apply coerce_env_full_cons ; auto with coc;
+  eauto with coc ecoc).
+  assert(coerce_in_env_full (A :: e) (A :: f)) by
+  (apply coerce_env_full_cons ; auto with coc;
+  eauto with coc ecoc).
+  apply tposr_coerce_prod with s ; eauto with coc ecoc.
+
+  assert(coerce_in_env_full (A' :: e) (A' :: f)) by
+  (apply coerce_env_full_cons ; auto with coc;
+  eauto with coc ecoc).
+  assert(coerce_in_env_full (A :: e) (A :: f)) by
+  (apply coerce_env_full_cons ; auto with coc;
+  eauto with coc ecoc).
+  apply tposr_coerce_sum with s s' ; eauto with coc ecoc.
+
+  assert(coerce_in_env_full (U :: e) (U :: f)) by
+  (apply coerce_env_full_cons ; auto with coc;
+  eauto with coc ecoc).
+  apply tposr_coerce_sub_l ; eauto with coc ecoc.
+
+  assert(coerce_in_env_full (U' :: e) (U' :: f)) by
+  (apply coerce_env_full_cons ; auto with coc ; eauto with coc ecoc).
+  apply tposr_coerce_sub_r ; eauto with coc ecoc.
+  
+  apply tposr_coerce_trans with B ; auto.
+Qed.
+
