proof/TPOSR/SubstitutionTPOSR.v
@@ -10,6 +10,7 @@ Require Import Lambda.TPOSR.LeftReflexivity.
 Require Import Lambda.TPOSR.Thinning.
 Require Import Lambda.TPOSR.CtxReduction.
 Require Import Lambda.TPOSR.CtxExpansion.
+Require Import Lambda.TPOSR.CtxCoercion.
 Require Import Lambda.TPOSR.Substitution.
 
 Require Import Coq.Arith.Lt.
@@ -41,15 +42,51 @@ Proof.
   clear IHsub_in_lenv ; intuition.
 Qed.
 
+Lemma wf_coerce : forall e, tposr_wf e -> coerce_in_env_full e e.
+Proof.
+  induction 1 ; simpl ; intros ; auto with coc.
+  apply coerce_env_in_env.
+  apply coerce_env_hd with s ; eauto with coc.
+Qed.  
+
+Lemma coerce_env_full_cons_coerce : forall G D, coerce_in_env_full G D -> 
+  forall T U s, G |-- T >-> U : s -> G |-- T -> T : s -> G |-- U -> U : s ->
+  coerce_in_env_full (T :: G) (U :: D).
+Proof.
+  induction 1 ; simpl ; intros.
+
+  apply coerce_env_trans with (U :: f) ; eauto with coc.
+  apply coerce_env_full_cons ; auto with coc.
+  apply wf_cons with s ; eauto with coc.
+  apply coerce_env_full with e ; auto.
+
+  apply coerce_env_trans with (T :: f).
+  apply coerce_env_in_env ; eauto with coc.
+
+  apply coerce_env_in_env ; eauto with coc.
+  apply coerce_env_hd with s ; eauto with coc.
+  apply coerce_coerce_env with e ; eauto with coc.
+  apply tposr_coerce_env with e ; eauto with coc.
+  apply tposr_coerce_env with e ; eauto with coc.
+  
+  apply coerce_env_in_env ; auto with coc.
+  apply coerce_env_hd with s ; auto with coc.
+Qed.
+
 Lemma ind_substitution_tposr : 
    (forall e t u U, e |-- t -> u : U ->
    forall g d d' T, g |-- d -> d' : T -> g |-- d' -> d' : T ->
    forall f n, sub_in_lenv d T n e f -> trunc _ n f g -> 
-   f |-- (lsubst_rec d t n) -> (lsubst_rec d' u n) : (lsubst_rec d U n)) /\
+   f |-- (lsubst_rec d t n) -> (lsubst_rec d' u n) : (lsubst_rec d U n) /\
+   exists f', sub_in_lenv d' T n e f' /\ trunc _ n f' g /\
+   tposr_wf f' /\ coerce_in_env_full f f') /\
    (forall e, tposr_wf e ->
    forall g d d' T, g |-- d -> d' : T -> g |-- d' -> d' : T ->
    forall n f, sub_in_lenv d T n e f -> trunc _ n f g -> 
-   tposr_wf f) /\
+   tposr_wf f /\
+   exists f', sub_in_lenv d' T n e f' /\ trunc _ n f' g /\
+   tposr_wf f' /\ coerce_in_env_full f f'
+   ) /\
    (forall e t u s, e |-- t ~= u : s ->
    forall g d d' T, g |-- d -> d' : T -> g |-- d' -> d' : T ->
    forall f n, sub_in_lenv d T n e f -> trunc _ n f g -> 
@@ -65,11 +102,15 @@ apply ind_tposr_wf_eq_coerce with
    (P:=fun e t u U => fun H : e |-- t -> u : U =>
    forall g d d' T, g |-- d -> d' : T -> g |-- d' -> d' : T ->
    forall f n, sub_in_lenv d T n e f -> trunc _ n f g -> 
-   f |-- (lsubst_rec d t n) -> (lsubst_rec d' u n) : (lsubst_rec d U n))
+   f |-- (lsubst_rec d t n) -> (lsubst_rec d' u n) : (lsubst_rec d U n) /\
+   exists f', sub_in_lenv d' T n e f' /\ trunc _ n f' g /\
+   tposr_wf f' /\ coerce_in_env_full f f')
    (P0:= fun e => fun H : tposr_wf e =>
    forall g d d' T, g |-- d -> d' : T -> g |-- d' -> d' : T ->
    forall n f, sub_in_lenv d T n e f -> trunc _ n f g -> 
-   tposr_wf f)
+   tposr_wf f /\
+   exists f', sub_in_lenv d' T n e f' /\ trunc _ n f' g /\
+   tposr_wf f' /\ coerce_in_env_full f f')
    (P1 := fun e t u s => fun H : e |-- t ~= u : s =>
    forall g d d' T, g |-- d -> d' : T -> g |-- d' -> d' : T ->
    forall f n, sub_in_lenv d T n e f -> trunc _ n f g -> 
@@ -83,6 +124,7 @@ apply ind_tposr_wf_eq_coerce with
    simpl in |- *;
    intros; auto with coc core arith datatypes.
 
+split.
 elim (lt_eq_lt_dec n0 n); [ intro Hlt_eq | intro Hlt ].
 elim i.
 elim Hlt_eq; clear Hlt_eq.
@@ -93,7 +135,7 @@ simpl in |- *.
 rewrite H4.
 rewrite simpl_lsubst; auto with coc core arith datatypes.
 apply tposr_var; auto with coc core arith datatypes.
-apply (H _ _ _ _ H0 H1 _ _ H2) ; auto.
+destruct (H _ _ _ _ H0 H1 _ _ H2) ; auto.
 exists x; auto with coc core arith datatypes.
 apply nth_sub_sup with d T0 n0 e; auto with coc core arith datatypes.
 
@@ -104,91 +146,177 @@ rewrite simpl_lsubst; auto with coc core arith datatypes.
 replace x with T0.
 apply thinning_n with g; auto with coc core arith datatypes.
 subst.
-apply (H _ _ _ _ H0 H1 _ _ H2) ; auto.
+destruct (H _ _ _ _ H0 H1 _ _ H2) ; auto.
 
 apply fun_item with e n; auto with coc core arith datatypes.
 apply nth_sub_eq with d f; auto with coc core arith datatypes.
 elim Heq; auto with coc core arith datatypes.
 
 apply tposr_var; auto with coc core arith datatypes.
-apply (H _ _ _ _ H0 H1 _ _ H2) ; auto.
+destruct (H _ _ _ _ H0 H1 _ _ H2) ; auto.
 apply nth_sub_inf with T0 e; auto with coc core arith datatypes.
 
-apply tposr_set ; eauto with coc.
+destruct (H _ _ _ _ H0 H1 _ _ H2) ; auto.
+destruct (H _ _ _ _ H0 H1 _ _ H2) ; auto.
+split ; [apply tposr_set|idtac] ; eauto with coc.
 
-apply tposr_prop ; eauto with coc.
+destruct (H _ _ _ _ H0 H1 _ _ H2) ; auto.
+split ; [apply tposr_prop|idtac] ; eauto with coc.
 
-apply tposr_prod with s1 ; eauto with coc ecoc core arith datatypes.
-
-apply tposr_abs with s1 (lsubst_rec d' B' (S n)) s2 ; eauto with coc core arith datatypes.
-
-rewrite distr_lsubst ; auto with coc.
-apply tposr_app with (lsubst_rec d A n) (lsubst_rec d A' n) s1 s2; eauto with coc core arith datatypes.
+destruct (H _ _ _ _ H1 H2 _ _ H3 H4).
+split ; auto.
 assert(sub_in_lenv d T (S n) (A :: e) (lsubst_rec d A n :: f)).
 apply sub_S ; auto with coc.
 assert(trunc lterm (S n) (lsubst_rec d A n :: f) g).
 apply trunc_S ; auto with coc.
-destruct (H0 _ _ _ _ H3 H4 _ _ H7 H8) ; auto with coc.
+destruct (H0 _ _ _ _ H1 H2 _ _ H7 H8) ; auto.
+apply tposr_prod with s1 ; eauto with coc ecoc core arith datatypes.
+
+destruct (H _ _ _ _ H2 H3 _ _ H4 H5).
+split ; auto.
+assert(sub_in_lenv d T (S n) (A :: e) (lsubst_rec d A n :: f)).
+apply sub_S ; auto with coc.
+assert(trunc lterm (S n) (lsubst_rec d A n :: f) g).
+apply trunc_S ; auto with coc.
+destruct (H1 _ _ _ _ H2 H3 _ _ H8 H9) ; auto.
+destruct (H0 _ _ _ _ H2 H3 _ _ H8 H9) ; auto.
+apply tposr_abs with s1 (lsubst_rec d' B' (S n)) s2 ; eauto with coc core arith datatypes.
+
+destruct (H _ _ _ _ H3 H4 _ _ H5 H6).
+split ; auto.
+rewrite distr_lsubst ; auto with coc.
+destruct (H2 _ _ _ _ H3 H4 _ _ H5 H6).
+destruct (H1 _ _ _ _ H3 H4 _ _ H5 H6).
+assert(sub_in_lenv d T (S n) (A :: e) (lsubst_rec d A n :: f)).
+apply sub_S ; auto with coc.
+assert(trunc lterm (S n) (lsubst_rec d A n :: f) g).
+apply trunc_S ; auto with coc.
+destruct (H0 _ _ _ _ H3 H4 _ _ H13 H14).
+destruct (H _ _ _ _ (refl_l H3) (refl_l H3) _ _ H5 H6).
+apply tposr_app with (lsubst_rec d A n) (lsubst_rec d A' n) s1 s2; eauto with coc core arith datatypes.
 
 rewrite distr_lsubst ; auto with coc.
 rewrite distr_lsubst ; auto with coc.
+destruct (H _ _ _ _ H3 H4 _ _ H5 H6).
+split ; auto.
+destruct (H2 _ _ _ _ H3 H4 _ _ H5 H6).
+assert(sub_in_lenv d T (S n) (A :: e) (lsubst_rec d A n :: f)).
+apply sub_S ; auto with coc.
+assert(trunc lterm (S n) (lsubst_rec d A n :: f) g).
+apply trunc_S ; auto with coc.
+destruct (H0 _ _ _ _ H3 H4 _ _ H11 H12).
+destruct (H1 _ _ _ _ H3 H4 _ _ H11 H12).
 apply tposr_beta with (lsubst_rec d' A' n) s1  (lsubst_rec d' B' (S n)) s2; eauto with coc core arith datatypes.
 
+destruct (H _ _ _ _ H1 H2 _ _ H3 H4).
+split ; auto.
 apply tposr_conv with (lsubst_rec d A n) s; eauto with coc.
 apply substitution_coerce_n with g T e ; eauto with coc.
 
+destruct (H _ _ _ _ H1 H2 _ _ H3 H4).
+split ; eauto with coc.
+assert(sub_in_lenv d T (S n) (A :: e) (lsubst_rec d A n :: f)).
+apply sub_S ; auto with coc.
+assert(trunc lterm (S n) (lsubst_rec d A n :: f) g).
+apply trunc_S ; auto with coc.
+destruct (H0 _ _ _ _ H1 H2 _ _ H7 H8).
 apply tposr_subset ; eauto with coc.
 
+destruct (H _ _ _ _ H1 H2 _ _ H3 H4).
+split ; auto.
+assert(sub_in_lenv d T (S n) (A :: e) (lsubst_rec d A n :: f)).
+apply sub_S ; auto with coc.
+assert(trunc lterm (S n) (lsubst_rec d A n :: f) g).
+apply trunc_S ; auto with coc.
+destruct (H0 _ _ _ _ H1 H2 _ _ H7 H8) ; auto with coc.
 apply tposr_sum with s1 s2; eauto with coc core arith datatypes.
 
+destruct (H _ _ _ _ H3 H4 _ _ H5 H6).
+split ; auto.
+assert(sub_in_lenv d T (S n) (A :: e) (lsubst_rec d A n :: f)).
+apply sub_S ; auto with coc.
+assert(trunc lterm (S n) (lsubst_rec d A n :: f) g).
+apply trunc_S ; auto with coc.
+destruct (H2 _ _ _ _ H3 H4 _ _ H5 H6).
+destruct (H1 _ _ _ _ H3 H4 _ _ H5 H6).
+destruct (H0 _ _ _ _ H3 H4 _ _ H9 H10).
 apply tposr_pair with s1 s2 s3 ; eauto with coc.
 rewrite <- distr_lsubst ; eauto with coc.
 
-pose (H _ _ _ _ H3 H4 _ _ H5 H6).
+destruct (H _ _ _ _ H3 H4 _ _ H5 H6).
+split ; auto.
 destruct (H0 _ _ _ _ H3 H4 _ _ H5 H6) ; auto with coc.
 assert(sub_in_lenv d T (S n) (A :: e) (lsubst_rec d A n :: f)).
 apply sub_S ; auto with coc.
 assert(trunc lterm (S n) (lsubst_rec d A n :: f) g).
 apply trunc_S ; auto with coc.
-destruct (H1 _ _ _ _ H3 H4 _ _ H9 H10) ; auto with coc.
+destruct (H1 _ _ _ _ H3 H4 _ _ H11 H12) ; auto with coc.
+destruct (H2 _ _ _ _ H3 H4 _ _ H5 H6) ; auto with coc.
 apply tposr_pi1 with s1 s2 s3 ; eauto with coc.
 
+destruct (H _ _ _ _ H3 H4 _ _ H5 H6).
+split ; auto.
+assert(sub_in_lenv d T (S n) (A :: e) (lsubst_rec d A n :: f)).
+apply sub_S ; auto with coc.
+assert(trunc lterm (S n) (lsubst_rec d A n :: f) g).
+apply trunc_S ; auto with coc.
+destruct (H0 _ _ _ _ H3 H4 _ _ H9 H10) ; auto with coc.
+destruct (H1 _ _ _ _ H3 H4 _ _ H5 H6) ; auto with coc.
+destruct (H2 _ _ _ _ H3 H4 _ _ H5 H6) ; auto with coc.
 apply tposr_pi1_red with (lsubst_rec d' A' n) s1 (lsubst_rec d' B' (S n))  s2 s3 (lsubst_rec d' v' n); eauto with coc.
 rewrite <- distr_lsubst.
 eauto with coc.
 
 rewrite distr_lsubst.
 simpl.
-pose (H _ _ _ _ H3 H4 _ _ H5 H6).
+destruct (H _ _ _ _ H3 H4 _ _ H5 H6).
+split ; auto.
 destruct (H0 _ _ _ _ H3 H4 _ _ H5 H6) ; auto with coc.
 assert(sub_in_lenv d T (S n) (A :: e) (lsubst_rec d A n :: f)).
 apply sub_S ; auto with coc.
 assert(trunc lterm (S n) (lsubst_rec d A n :: f) g).
 apply trunc_S ; auto with coc.
-destruct (H1 _ _ _ _ H3 H4 _ _ H9 H10) ; auto with coc.
+destruct (H1 _ _ _ _ H3 H4 _ _ H11 H12) ; auto with coc.
+destruct (H2 _ _ _ _ H3 H4 _ _ H5 H6) ; auto with coc.
 apply tposr_pi2 with s1 s2 s3 ; eauto with coc.
 
 rewrite distr_lsubst.
 simpl.
+destruct (H _ _ _ _ H3 H4 _ _ H5 H6).
+split ; auto.
+
+assert(sub_in_lenv d T (S n) (A :: e) (lsubst_rec d A n :: f)).
+apply sub_S ; auto with coc.
+assert(trunc lterm (S n) (lsubst_rec d A n :: f) g).
+apply trunc_S ; auto with coc.
+destruct (H0 _ _ _ _ H3 H4 _ _ H9 H10) ; auto with coc.
+destruct (H1 _ _ _ _ H3 H4 _ _ H5 H6) ; auto with coc.
+destruct (H2 _ _ _ _ H3 H4 _ _ H5 H6) ; auto with coc.
 apply tposr_pi2_red with (lsubst_rec d' A' n) s1 (lsubst_rec d' B' (S n))  s2 s3 (lsubst_rec d' u' n); eauto with coc.
 rewrite <- distr_lsubst ; eauto with coc.
 
 inversion H1.
 inversion H2 ; subst.
-apply (wf_tposr t).
+assert(tposr_wf f) by apply (wf_tposr t).
+split ; auto.
+exists f.
+split ; intuition.
+apply (wf_coerce H4).
+
 inversion H3.
-apply wf_cons with (lsubst_rec d' A' n0) s ; apply (H _ _ _ _ H0 H1 _ _ H8 H9).
-
-split ; eauto with coc ecoc.
-apply tposr_eq_trans with (lsubst_rec d X n) ; eauto with coc.
-apply tposr_eq_sym.
-apply tposr_eq_tposr.
-eapply H ; eauto with coc.
-eapply H ; eauto with coc.
-apply substitution_eq_n with g T e ; eauto with coc.
-
-destruct (H _ _ _ _ H0 H1 _ _ H2 H3).
-intuition.
+destruct (H _ _ _ _ H0 H1 _ _ H8 H9).
+split ; auto.
+destruct (H _ _ _ _ (refl_l H0) (refl_l H0) _ _ H8 H9).
+subst.
+apply wf_cons with s ; auto.
+destruct H11 ; destruct_exists.
+exists (lsubst_rec d' A n0 :: x0).
+subst.
+destruct (H _ _ _ _ H1 H1 _ _ H11 H12).
+intuition ; auto with coc.
+apply wf_cons with s ; auto with coc.
+apply coerce_env_full_cons_coerce with s ; eauto with coc.
+apply coerce_env_full with x0 ; eauto with coc ecoc.
 
 destruct (H _ _ _ _ H1 H2 _ _ H3 H4).
 destruct (H0 _ _ _ _ H1 H2 _ _ H3 H4).
@@ -199,8 +327,16 @@ split.
 apply tposr_eq_trans with (lsubst_rec d X n) ; eauto with coc.
 apply tposr_eq_trans with (lsubst_rec d X n) ; eauto with coc.
 
-destruct (H _ _ _ _ H0 H1 _ _ H2 H3).
-auto with coc.
+destruct (H _ _ _ _ H0 H1 _ _ H2 H3) ; auto with coc.
+
+destruct (H _ _ _ _ H1 H2 _ _ H3 H4).
+destruct (H0 _ _ _ _ H1 H2 _ _ H3 H4).
+destruct (H _ _ _ _ (refl_l H1) (refl_l H1) _ _ H3 H4).
+destruct (H0 _ _ _ _ (refl_l H1) (refl_l H1) _ _ H3 H4).
+
+split ; apply tposr_eq_trans with (lsubst_rec d X n) ; eauto with coc.
+
+destruct (H _ _ _ _ H0 H1 _ _ H2 H3) ; auto with coc.
 
 destruct (H _ _ _ _ H3 H4 _ _ H5 H6).
 assert(sub_in_lenv d T (S n) (A' :: e) (lsubst_rec d A' n :: f)).
@@ -208,70 +344,112 @@ apply sub_S ; auto with coc.
 assert(trunc lterm (S n) (lsubst_rec d A' n :: f) g).
 apply trunc_S ; auto with coc.
 destruct (H2 _ _ _ _ H3 H4 _ _ H9 H10) ; auto with coc.
-split ; apply tposr_coerce_prod with s ; eauto with coc.
-destruct (sub_red_env H3 H4 H5 H6).
+destruct (H0 _ _ _ _ H3 H4 _ _ H5 H6).
 destruct_exists.
-pose (H0 _ _ _ _ H4 H4 _ _ H13 H14).
-apply tposr_exp_env with x ; auto with coc.
-
-Focus 5.
-destruct (H _ _ _ _ H3 H4 _ _ H5 H6).
-assert(sub_in_lenv d T (S n) (U :: e) (lsubst_rec d U n :: f)).
-apply sub_S ; auto with coc.
-assert(trunc lterm (S n) (lsubst_rec d U n :: f) g).
-apply trunc_S ; auto with coc.
-pose (H0 _ _ _ _(refl_l H3) (refl_l H3) _ _ H5 H6).
-
-split ; apply tposr_coerce_sub_l ; auto with coc ecoc.
-apply tposr_coerce_conv.
-apply tposr_eq_tposr ; auto with coc.
-eauto with coc ecoc.
-
-Admitted.
-
-
-
-(*
-
-pose
-
-apply 
-coerce_red_env with (lsubst_rec d A' n :: f) ; auto with coc.
-apply red_env_hd with s.
-eapply H0 ; eauto with coc.
-
-
-split.
-destruct (H _ _ _ _ H3 H4 _ _ H5 H6).
-apply tposr_coerce_sub_l ; eauto with coc.
-Focus 2.
-destruct (H _ _ _ _ H3 H4 _ _ H5 H6).
-assert(sub_in_lenv d T (S n) (U :: e) (lsubst_rec d U n :: f)).
-apply sub_S ; auto with coc.
-assert(trunc lterm (S n) (lsubst_rec d U n :: f) g).
-apply trunc_S ; auto with coc.
-pose (H2 _ _ _ _ H3 H4 _ _ H9 H10).
-apply tposr_coerce_sub_l ; eauto with coc.
-Focus 2.
+destruct (H0 _ _ _ _ H4 H4 _ _ H14 H15).
+destruct (H1 _ _ _ _ (refl_l H3) (refl_l H3) _ _ H5 H6) ; auto.
+destruct (H1 _ _ _ _  H3 H4 _ _ H5 H6) ; auto.
+destruct (H1 _ _ _ _  H4 H4 _ _ H14 H15) ; auto.
 split ; apply tposr_coerce_prod with s ; auto with coc.
 
-  
+apply coerce_env_full with x ; auto with coc.
 
-
-apply substitution_sorted_n with g T e ; auto with coc.
-
-
-apply tposr_coerce_sum with s s' ; eauto with coc.
-
-apply tposr_coerce_sub_l ; eauto with coc.
-
-apply tposr_coerce_sub_r ; eauto with coc.
-
+apply coerce_red_env with (lsubst_rec d A' n :: f) ; auto with coc.
+apply red_env_hd with s ; auto.
+apply coerce_env_full with x ; auto with coc.
 eauto with coc.
+apply coerce_env_full with x ; auto with coc.
+
+destruct (H _ _ _ _ H3 H4 _ _ H5 H6).
+assert(sub_in_lenv d T (S n) (A :: e) (lsubst_rec d A n :: f)).
+apply sub_S ; auto with coc.
+assert(trunc lterm (S n) (lsubst_rec d A n :: f) g).
+apply trunc_S ; auto with coc.
+destruct (H2 _ _ _ _ H3 H4 _ _ H9 H10) ; auto with coc.
+destruct (H0 _ _ _ _ H3 H4 _ _ H5 H6).
+destruct_exists.
+destruct (H0 _ _ _ _ H4 H4 _ _ H14 H15).
+destruct (H1 _ _ _ _ (refl_l H3) (refl_l H3) _ _ H5 H6) ; auto.
+destruct (H0 _ _ _ _ (refl_l H3) (refl_l H3) _ _ H5 H6) ; auto.
+destruct (H1 _ _ _ _  H3 H4 _ _ H5 H6) ; auto.
+destruct (H1 _ _ _ _  H4 H4 _ _ H14 H15) ; auto.
+split ; apply tposr_coerce_sum with s s' ; auto with coc.
+
+apply coerce_env_full with x ; auto with coc.
+destruct (H0 _ _ _ _ (refl_l H3) (refl_l H3) _ _ H5 H6) ; auto.
+apply coerce_env_full with x ; auto with coc.
+
+apply coerce_red_env with (lsubst_rec d A n :: f) ; auto with coc.
+apply red_env_hd with s ; auto.
+apply coerce_env_full with x ; auto with coc.
+
+destruct (H _ _ _ _ H3 H4 _ _ H5 H6).
+assert(sub_in_lenv d T (S n) (U :: e) (lsubst_rec d U n :: f)).
+apply sub_S ; auto with coc.
+assert(trunc lterm (S n) (lsubst_rec d U n :: f) g).
+apply trunc_S ; auto with coc.
+destruct (H2 _ _ _ _ H3 H4 _ _ H9 H10) ; auto with coc.
+destruct (H0 _ _ _ _ H3 H4 _ _ H5 H6).
+destruct_exists.
+destruct (H0 _ _ _ _ H4 H4 _ _ H14 H15).
+destruct (H1 _ _ _ _ (refl_l H3) (refl_l H3) _ _ H5 H6) ; auto.
+destruct (H0 _ _ _ _ (refl_l H3) (refl_l H3) _ _ H5 H6) ; auto.
+destruct (H1 _ _ _ _  H3 H4 _ _ H5 H6) ; auto.
+destruct (H1 _ _ _ _  H4 H4 _ _ H14 H15) ; auto.
+
+split ; 
+apply tposr_coerce_sub_l ; eauto with coc.
+apply coerce_env_full with x ; auto with coc.
+apply coerce_env_full with x ; auto with coc.
+
+change (Srt_l prop) with (lsubst_rec d' (Srt_l prop) (S n)).
+assert(sub_in_lenv d' T (S n) (U :: e) (lsubst_rec d' U n :: x)).
+apply sub_S ; auto with coc.
+assert(trunc lterm (S n) (lsubst_rec d' U n :: x) g).
+apply trunc_S ; auto with coc.
+destruct(H2 _ _ _ _ H4 H4 _ _ H31 H32).
+apply coerce_env_full with (lsubst_rec d' U n :: x) ; auto.
+apply coerce_env_full_cons ; auto with coc.
+apply wf_cons with set ; auto.
+
+destruct (H _ _ _ _ H3 H4 _ _ H5 H6).
+assert(sub_in_lenv d T (S n) (U' :: e) (lsubst_rec d U' n :: f)).
+apply sub_S ; auto with coc.
+assert(trunc lterm (S n) (lsubst_rec d U' n :: f) g).
+apply trunc_S ; auto with coc.
+destruct (H2 _ _ _ _ H3 H4 _ _ H9 H10) ; auto with coc.
+destruct (H0 _ _ _ _ H3 H4 _ _ H5 H6).
+destruct_exists.
+destruct (H0 _ _ _ _ H4 H4 _ _ H14 H15).
+destruct (H1 _ _ _ _ H4 H4 _ _ H14 H15).
+destruct (H1 _ _ _ _ (refl_l H3) (refl_l H3) _ _ H5 H6).
+
+split ; 
+apply tposr_coerce_sub_r ; eauto with coc.
+apply coerce_env_full with x ; auto with coc.
+
+change (Srt_l prop) with (lsubst_rec d' (Srt_l prop) (S n)).
+assert(sub_in_lenv d' T (S n) (U' :: e) (lsubst_rec d' U' n :: x)).
+apply sub_S ; auto with coc.
+assert(trunc lterm (S n) (lsubst_rec d' U' n :: x) g).
+apply trunc_S ; auto with coc.
+destruct(H2 _ _ _ _ H4 H4 _ _ H27 H28).
+apply coerce_env_full with (lsubst_rec d' U' n :: x) ; auto.
+apply coerce_env_full_cons ; auto with coc.
+apply wf_cons with set ; auto.
+apply coerce_env_full with x ; auto with coc.
+
+destruct (H _ _ _ _ H0 H1 _ _ H2 H3) ; intuition.
+
+destruct (H _ _ _ _ H1 H2 _ _ H3 H4) ;
+destruct (H0 _ _ _ _ H1 H2 _ _ H3 H4) ;
+destruct (H0 _ _ _ _ (refl_l H1) (refl_l H1) _ _ H3 H4) ;
+destruct (H _ _ _ _ (refl_l H1) (refl_l H1) _ _ H3 H4) ;
+intuition.
 
 apply tposr_coerce_trans with (lsubst_rec d B n) ; eauto with coc.
+apply tposr_coerce_trans with (lsubst_rec d B n) ; eauto with coc.
 Qed.
-*)
 
 Corollary substitution_tposr_tposr_n : forall g d d' t, g |-- d -> d' : t -> g |-- d' -> d' : t ->
    forall e u v U, e |-- u -> v : U ->
@@ -279,7 +457,8 @@ Corollary substitution_tposr_tposr_n : forall g d d' t, g |-- d -> d' : t -> g |
    f |-- (lsubst_rec d u n) -> (lsubst_rec d' v n) : (lsubst_rec d U n).
 Proof.
   intros.
-  eapply (proj1 (ind_substitution_tposr)) ; eauto with coc.
+  pose (proj1 (ind_substitution_tposr)).
+  pose (a _ _ _ _ H1 _ _ _ _ H H0 _ _  H2 H3) ; intuition ; eauto with coc.
 Qed.
 
 Corollary substitution_tposr_tposr_wf_n : forall g d d' t, g |-- d -> d' : t -> g |-- d' -> d' : t ->
@@ -287,7 +466,8 @@ Corollary substitution_tposr_tposr_wf_n : forall g d d' t, g |-- d -> d' : t -> 
    trunc _ n f g -> tposr_wf f.
 Proof.
   intros.
-  apply (proj1 (proj2 (ind_substitution_tposr))) with e g d d' t n ; eauto with coc.
+  pose (proj1 (proj2 (ind_substitution_tposr))).
+  pose (a _ H1 _ _ _ _ H H0 _ _  H2 H3) ; intuition ; eauto with coc.
 Qed.
 
 Corollary substitution_tposr_eq_n : forall g d d' t, g |-- d -> d' : t -> g |-- d' -> d' : t ->
